---
tags:
  - Math
  - AGLA
---
$$\Large(\overline r - \overline r_0,\overline n) = 0$$

---

$(\overline r - \overline r_0,\overline n) = (\overline r,\overline n)-(\overline r_0,\overline n) = 0$
$(\overline r,\overline n) = Ax+By+Cz \iff \overline n = \left(\begin{matrix}A\\ B\\ C\end{matrix}\right)\;\&\;\overline r = \left(\begin{matrix}x\\ y\\ z\end{matrix}\right)$
$(\overline r_0,\overline n) = Ax_0+By_0+Cz_0\iff\overline n = \left(\begin{matrix}A\\ B\\ C\end{matrix}\right)\;\&\;\overline r_0 = \left(\begin{matrix}x_0\\ y_0\\ z_0\end{matrix}\right)$

$(\overline r - \overline r_0,\overline n) = Ax+By+Cz-Ax_0-By_0-Cz_0=Ax+By+Cz+D$ ([[General Equation of a Plane]])